complete progress proof for arith

arith.lean
@@ -3,110 +3,457 @@
 section arith
 
 inductive typ : Type
-  | numt : typ
-  | boolt : typ
+  | num : typ
+  | bool : typ
 
-instance : decidable_eq typ := by tactic.mk_dec_eq_instance
-
-inductive val : Type
-  | numv : ℕ → val
-  | boolv : bool → val
-
+lemma typ_cases {p: Prop} (t: typ)
+    (num_case: t = typ.num → p)
+    (bool_case: t = typ.bool → p): p :=
+  begin
+    induction t,
+    case typ.num {
+      apply num_case rfl
+    },
+    case typ.bool {
+      apply bool_case rfl
+    }
+  end
 
 inductive exp : Type
-  | value : val → exp
+  | num : ℕ → exp
+  | bool : bool → exp
   | add : exp → exp → exp
   | ite : exp → exp → exp → exp
   | eq : exp → exp → exp
 
-open typ
-open val
-open exp
+inductive is_value : exp → Prop
+  | num {n: ℕ} : is_value (exp.num n)
+  | bool {b: bool} : is_value (exp.bool b)
 
-def is_val (e: exp): Prop := ∃v: val, e = value v
+lemma is_value_cases {p: Prop} {e: exp} (e_is_value: is_value e)
+    (num_case: ∀ (n: ℕ), e = exp.num n → p)
+    (bool_case: ∀ (b: bool), e = exp.bool b → p): p :=
+  begin
+    induction e_is_value,
+    case is_value.num n {
+      apply num_case n rfl
+    },
+    case is_value.bool b {
+      apply bool_case b rfl
+    }
+  end
 
-def step : exp → option exp
-  | (add (value (numv v1)) (value (numv v2))) :=
-      some (value (numv (v1 + v2)))
-  | (add (value v1) e2) :=
-      do e2' ← step e2,
-         return $ add (value v1) e2'
-  | (add e1 e2) :=
-      do e1' ← step e1,
-         return $ add e1' e2
-  | (ite (value (boolv tt)) e1 e2) :=
-      some e1
-  | (ite (value (boolv ff)) e1 e2) :=
-      some e2
-  | (ite e1 e2 e3) :=
-      do e1' ← step e1,
-         return $ (ite e1 e2 e3)
-  | (eq (value (numv v1)) (value (numv v2))) :=
-      some (value (boolv (v1 = v2)))
-  | (eq (value (boolv b1)) (value (boolv b2))) :=
-      some (value (boolv (b1 = b2)))
-  | (eq (value v1) e2) :=
-      do e2' ← step e2,
-         return $ eq (value v1) e2'
-  | (eq e1 e2) :=
-      do e1' ← step e1,
-         return $ eq e1' e2
-  | _ :=
-      none
+inductive step : exp → exp → Prop
+  notation e1 `⟶` e2:100 := step e1 e2
+  | add {n1 n2: ℕ}:             exp.add (exp.num n1) (exp.num n2) ⟶ exp.num (n1 +n2)
+  | add_right {e1 e2 e2': exp}: is_value e1 → (e2 ⟶ e2') →
+                                (exp.add e1 e2 ⟶ exp.add e1 e2')
+  | add_left {e1 e1' e2: exp}:  (e1 ⟶ e1') →
+                                (exp.add e1 e2 ⟶ exp.add e1' e2)
+  | ite_true {e2 e3: exp}:      exp.ite (exp.bool true) e2 e3 ⟶ e2
+  | ite_false {e2 e3: exp}:     exp.ite (exp.bool false) e2 e3 ⟶ e3
+  | ite {e1 e1' e2 e3: exp}:    (e1 ⟶ e1') →
+                                (exp.ite e1 e2 e3 ⟶ exp.ite e1' e2 e3)
+  | eq_num {n1 n2: ℕ}:          exp.eq (exp.num n1) (exp.num n2) ⟶ exp.bool (n1 = n2)
+  | eq_bool {b1 b2: bool}:      exp.eq (exp.bool b1) (exp.bool b2) ⟶ exp.bool (b1 = b2)
+  | eq_right {e1 e2 e2': exp}:  is_value e1 → (e2 ⟶ e2') →
+                                (exp.eq e1 e2 ⟶ exp.eq e1 e2')
+  | eq_left {e1 e1' e2: exp}:   (e1 ⟶ e1') →
+                                (exp.eq e1 e2 ⟶ exp.eq e1' e2)
 
-reserve infixl `:::`:50
+notation e1 `⟶` e2:100 := step e1 e2
 
 inductive typed : exp → typ → Prop
-  | t_num (n: ℕ) : typed (value (numv n)) numt
-  | t_bool (b: bool) : typed (value (boolv b)) boolt
-  | t_add (e1 e2: exp) : typed e1 numt → typed e2 numt → typed (add e1 e2) numt
-  | t_ite (e1 e2 e3: exp) {t: typ} : typed e1 boolt → typed e2 t → typed e3 t → typed (ite e1 e2 e3) t
-  | t_eq (e1 e2: exp) {t: typ} : typed e1 t → typed e2 t → typed (eq e1 e2) boolt
+  notation e1 `:::` e2:100 := typed e1 e2
+  | num {n: ℕ}:                   exp.num n ::: typ.num
+  | bool {b: bool}:               exp.bool b ::: typ.bool
+  | add {e1 e2: exp}:             (e1 ::: typ.num) → (e2 ::: typ.num) →
+                                  (exp.add e1 e2 ::: typ.num)
+  | ite {e1 e2 e3: exp} {t: typ}: (e1 ::: typ.bool) → (e2 ::: t) → (e3 ::: t) →
+                                  (exp.ite e1 e2 e3 ::: t)
+  | eq {e1 e2: exp} {t: typ}:     (e1 ::: t) → (e2 ::: t) →
+                                  (exp.eq e1 e2 ::: typ.bool)
 
-infixl `:::` := typed
+notation e1 `:::` e2:100 := typed e1 e2
 
-theorem progress(e: exp) (t: typ) (is_typed: typed e t): is_val e ∨ step e ≠ none :=
-  exp.rec_on e
-    (
-      assume v: val,
-      let e := value v in
-      have e_is_val: is_val e, from exists.intro v rfl,
-      show is_val e ∨ step e ≠ none, from or.inl e_is_val
+lemma typed_cases {p: Prop} {e: exp} {t: typ} (e_typed_t: e ::: t)
+    (num_case: ∀ (n: ℕ), e = exp.num n → t = typ.num → p)
+    (bool_case: ∀ (b: bool), e = exp.bool b → t = typ.bool → p)
+    (add_case: ∀ (e1 e2: exp), (e1 ::: typ.num) → (e2 ::: typ.num) → e = exp.add e1 e2 → t = typ.num → p)
+    (ite_case: ∀ (e1 e2 e3: exp), (e1 ::: typ.bool) → (e2 ::: t) → (e3 ::: t) → e = exp.ite e1 e2 e3 → p)
+    (eq_case: ∀ (e1 e2: exp) (t1: typ), (e1 ::: t1) → (e2 ::: t1) → e = exp.eq e1 e2 → t = typ.bool → p): p :=
+  begin
+    induction e_typed_t,
+    case typed.num n {
+      apply num_case n rfl rfl
+    },
+    case typed.bool b {
+      apply bool_case b rfl rfl
+    },
+    case typed.add e1 e2 e1_typed_num e2_typed_num {
+      apply add_case e1 e2 e1_typed_num e2_typed_num rfl rfl
+    },
+    case typed.ite e1 e2 e3 t1 e1_typed_bool e2_typed_t e3_typed_t {
+      apply ite_case e1 e2 e3 e1_typed_bool e2_typed_t e3_typed_t rfl
+    },
+    case typed.eq e1 e2 t1 e1_typed_t1 e2_typed_t1 {
+      apply eq_case e1 e2 t1 e1_typed_t1 e2_typed_t1 rfl rfl
+    },
+  end
+
+lemma numt_inversion {e: exp} (e_typed_num: e ::: typ.num) (e_is_val: is_value e): ∃n: ℕ, e = exp.num n :=
+  typed_cases e_typed_num
+  ( -- num
+    assume n: ℕ,
+    assume e_is_num: e = exp.num n,
+    assume _,
+    exists.intro n e_is_num 
+  )
+  ( -- bool
+    assume _ _,
+    assume numt_is_boolt: typ.num = typ.bool,
+    show ∃n: ℕ, e = exp.num n, from typ.no_confusion numt_is_boolt
+  )
+  ( -- add
+    assume e1 e2: exp,
+    assume _ _,
+    assume e_is_add: e = exp.add e1 e2,
+    assume _,
+    is_value_cases e_is_val
+    (  -- is value num
+      assume n: ℕ,
+      assume e_is_num: e = exp.num n,
+      have add_is_num: exp.add e1 e2 = exp.num n, from eq.trans (eq.symm e_is_add) e_is_num,
+      show ∃n: ℕ, e = exp.num n, from exp.no_confusion add_is_num
     )
-    (
-      assume e1 e2: exp,
-      assume e1ih: is_val e1 ∨ step e1 ≠ none,
-      assume e2ih: is_val e2 ∨ step e2 ≠ none,
-      let e := add e1 e2 in
-      or.elim e1ih (
-        assume e1_is_val: is_val e1,
-        or.elim e2ih (
-          assume e2_is_val: is_val e2,
+    (  -- is value bool
+      assume b: bool,
+      assume e_is_bool: e = exp.bool b,
+      have add_is_bool: exp.add e1 e2 = exp.bool b, from eq.trans (eq.symm e_is_add) e_is_bool,
+      show ∃n: ℕ, e = exp.num n, from exp.no_confusion add_is_bool
+    )
+  )
+  ( -- ite
+    assume e1 e2 e3: exp,
+    assume _ _ _,
+    assume e_is_ite: e = exp.ite e1 e2 e3,
+    is_value_cases e_is_val
+    (  -- is value num
+      assume n: ℕ,
+      assume e_is_num: e = exp.num n,
+      have add_is_num: exp.ite e1 e2 e3 = exp.num n, from eq.trans (eq.symm e_is_ite) e_is_num,
+      show ∃n: ℕ, e = exp.num n, from exp.no_confusion add_is_num
+    )
+    (  -- is value bool
+      assume b: bool,
+      assume e_is_bool: e = exp.bool b,
+      have add_is_bool: exp.ite e1 e2 e3 = exp.bool b, from eq.trans (eq.symm e_is_ite) e_is_bool,
+      show ∃n: ℕ, e = exp.num n, from exp.no_confusion add_is_bool
+    )
+  )
+  ( -- eq
+    assume e1 e2: exp,
+    assume _ _ _,
+    assume e_is_eq: e = exp.eq e1 e2,
+    assume _,
+    is_value_cases e_is_val
+    (  -- is value num
+      assume n: ℕ,
+      assume e_is_num: e = exp.num n,
+      have add_is_num: exp.eq e1 e2 = exp.num n, from eq.trans (eq.symm e_is_eq) e_is_num,
+      show ∃n: ℕ, e = exp.num n, from exp.no_confusion add_is_num
+    )
+    (  -- is value bool
+      assume b: bool,
+      assume e_is_bool: e = exp.bool b,
+      have add_is_bool: exp.eq e1 e2 = exp.bool b, from eq.trans (eq.symm e_is_eq) e_is_bool,
+      show ∃n: ℕ, e = exp.num n, from exp.no_confusion add_is_bool
+    )
+  )
 
-          show is_val e ∨ step e ≠ none, from sorry
-        ) (
-          assume e2_can_step: step e2 ≠ none,
-          show is_val e ∨ step e ≠ none, from sorry
+lemma boolt_inversion {e: exp} (e_typed_bool: e ::: typ.bool) (e_is_val: is_value e):
+                      e = exp.bool true ∨ e = exp.bool false :=
+  typed_cases e_typed_bool
+  ( -- num
+    assume _ _,
+    assume numt_is_boolt: typ.bool = typ.num,
+    show e = exp.bool true ∨ e = exp.bool false, from typ.no_confusion numt_is_boolt
+  )
+  ( -- bool
+    assume b: bool,
+    assume e_is_bool: e = exp.bool b,
+    assume : typ.bool = typ.bool,
+    show e = exp.bool true ∨ e = exp.bool false, by begin
+      cases b,
+      case tt {
+        apply or.inl,
+        assumption
+      },
+      case ff {
+        apply or.inr,
+        assumption
+      }
+    end
+  )
+  ( -- add
+    assume e1 e2: exp,
+    assume _ _,
+    assume e_is_add: e = exp.add e1 e2,
+    assume _,
+    is_value_cases e_is_val
+    (  -- is value num
+      assume n: ℕ,
+      assume e_is_num: e = exp.num n,
+      have add_is_num: exp.add e1 e2 = exp.num n, from eq.trans (eq.symm e_is_add) e_is_num,
+      show e = exp.bool true ∨ e = exp.bool false, from exp.no_confusion add_is_num
+    )
+    (  -- is value bool
+      assume b: bool,
+      assume e_is_bool: e = exp.bool b,
+      have add_is_bool: exp.add e1 e2 = exp.bool b, from eq.trans (eq.symm e_is_add) e_is_bool,
+      show e = exp.bool true ∨ e = exp.bool false, from exp.no_confusion add_is_bool
+    )
+  )
+  ( -- ite
+    assume e1 e2 e3: exp,
+    assume _ _ _,
+    assume e_is_ite: e = exp.ite e1 e2 e3,
+    is_value_cases e_is_val
+    (  -- is value num
+      assume n: ℕ,
+      assume e_is_num: e = exp.num n,
+      have add_is_num: exp.ite e1 e2 e3 = exp.num n, from eq.trans (eq.symm e_is_ite) e_is_num,
+      show e = exp.bool true ∨ e = exp.bool false, from exp.no_confusion add_is_num
+    )
+    (  -- is value bool
+      assume b: bool,
+      assume e_is_bool: e = exp.bool b,
+      have add_is_bool: exp.ite e1 e2 e3 = exp.bool b, from eq.trans (eq.symm e_is_ite) e_is_bool,
+      show e = exp.bool true ∨ e = exp.bool false, from exp.no_confusion add_is_bool
+    )
+  )
+  ( -- eq
+    assume e1 e2: exp,
+    assume _ _ _,
+    assume e_is_eq: e = exp.eq e1 e2,
+    assume _,
+    is_value_cases e_is_val
+    (  -- is value num
+      assume n: ℕ,
+      assume e_is_num: e = exp.num n,
+      have add_is_num: exp.eq e1 e2 = exp.num n, from eq.trans (eq.symm e_is_eq) e_is_num,
+      show e = exp.bool true ∨ e = exp.bool false, from exp.no_confusion add_is_num
+    )
+    (  -- is value bool
+      assume b: bool,
+      assume e_is_bool: e = exp.bool b,
+      have add_is_bool: exp.eq e1 e2 = exp.bool b, from eq.trans (eq.symm e_is_eq) e_is_bool,
+      show e = exp.bool true ∨ e = exp.bool false, from exp.no_confusion add_is_bool
+    )
+  )
+
+theorem progress(e: exp) (t: typ) (is_typed: e ::: t): is_value e ∨ ∃e', e ⟶ e' :=
+  typed.rec_on is_typed
+    ( -- num
+      assume n: ℕ,
+      let e := exp.num n in
+      have e_is_val: is_value e, from is_value.num,
+      show is_value e ∨ ∃e', e ⟶ e', from or.inl e_is_val
+    )
+    ( -- bool
+      assume b: bool,
+      let e := exp.bool b in
+      have e_is_val: is_value e, from is_value.bool,
+      show is_value e ∨ ∃e', e ⟶ e', from or.inl e_is_val
+    )
+    ( -- add
+      assume e1 e2: exp,
+      assume e1_is_numt : e1 ::: typ.num,
+      assume e2_is_numt : e2 ::: typ.num,
+      assume e1ih: is_value e1 ∨ ∃e1', e1 ⟶ e1',
+      assume e2ih: is_value e2 ∨ ∃e2', e2 ⟶ e2',
+      let e := exp.add e1 e2 in
+      have e_is_add: e = exp.add e1 e2, from rfl,
+      have e_steps: ∃e', e ⟶ e', from or.elim e1ih (
+        assume e1_is_val: is_value e1,
+        or.elim e2ih (
+          assume e2_is_val: is_value e2,
+          have e1_exists_num: ∃n1: ℕ, e1 = exp.num n1, from numt_inversion e1_is_numt e1_is_val,
+          have e2_exists_num: ∃n2: ℕ, e2 = exp.num n2, from numt_inversion e2_is_numt e2_is_val,
+          exists.elim e1_exists_num (
+            assume n1: ℕ,
+            assume e1_is_num: e1 = exp.num n1,
+            exists.elim e2_exists_num (
+              assume n2: ℕ,
+              assume e2_is_num: e2 = exp.num n2,
+              have exp.add (exp.num n1) (exp.num n2) ⟶ exp.num (n1 + n2), from step.add,
+              have e ⟶ exp.num (n1 + n2), by { rw [←e1_is_num, ←e2_is_num, ←e_is_add] at this, assumption },
+              show ∃e', e ⟶ e', from exists.intro (exp.num (n1 + n2)) this
+            )
+          )
         )
-      ) (
-        assume e1_can_step: step e1 ≠ none,
-        show is_val e ∨ step e ≠ none, from sorry
+        (
+          assume e2_can_step: ∃e2', e2 ⟶ e2',
+          exists.elim e2_can_step (
+            assume e2': exp,
+            assume e2_steps: e2 ⟶ e2',
+            have e ⟶ exp.add e1 e2', from step.add_right e1_is_val e2_steps,
+            show ∃e', e ⟶ e', from exists.intro (exp.add e1 e2') this
+          )
+        )
+      )
+      (
+        assume e1_can_step: ∃e1', e1 ⟶ e1',
+        exists.elim e1_can_step (
+          assume e1': exp,
+          assume e1_steps: e1 ⟶ e1',
+          have e ⟶ exp.add e1' e2, from step.add_left e1_steps,
+          show ∃e', e ⟶ e', from exists.intro (exp.add e1' e2) this
+        )
+      ),
+      show is_value e ∨ ∃e', e ⟶ e', from or.inr e_steps
+    )
+    ( -- ite
+      assume e1 e2 e3: exp,
+      assume t: typ,
+      assume e1_is_bool: e1 ::: typ.bool,
+      assume e2_is_t: e2 ::: t,
+      assume e3_is_t: e3 ::: t,
+      assume e1ih: is_value e1 ∨ ∃e1', e1 ⟶ e1',
+      assume e2ih: is_value e2 ∨ ∃e2', e2 ⟶ e2',
+      assume e3ih: is_value e3 ∨ ∃e3', e3 ⟶ e3',
+      let e := exp.ite e1 e2 e3 in
+      have e_is_ite: e = exp.ite e1 e2 e3, from rfl,
+      or.elim e1ih
+      ( -- is_value e1
+        assume e1_is_val: is_value e1,
+        have e1_bool: e1 = exp.bool true ∨ e1 = exp.bool false, from boolt_inversion e1_is_bool e1_is_val,
+        or.elim e1_bool
+        ( -- ite-true
+          assume e1_is_true: e1 = exp.bool true,
+          have exp.ite (exp.bool true) e2 e3 ⟶ e2, from step.ite_true,
+          have e ⟶ e2, by { rw [←e1_is_true, ←e_is_ite] at this, assumption },
+          have e_steps: ∃e', e ⟶ e', from exists.intro e2 this,
+          show is_value e ∨ ∃e', e ⟶ e', from or.inr e_steps
+        )
+        ( -- ite-false
+          assume e1_is_false: e1 = exp.bool false,
+          have exp.ite (exp.bool false) e2 e3 ⟶ e3, from step.ite_false,
+          have e ⟶ e3, by { rw [←e1_is_false, ←e_is_ite] at this, assumption },
+          have e_steps: ∃e', e ⟶ e', from exists.intro e3 this,
+          show is_value e ∨ ∃e', e ⟶ e', from or.inr e_steps
+        )
+      )
+      ( -- e1 steps
+        assume e1_can_step: ∃e1', e1 ⟶ e1',
+        exists.elim e1_can_step (λe1', 
+          assume e1_steps: e1 ⟶ e1',
+          have e ⟶ exp.ite e1' e2 e3, from step.ite e1_steps,
+          have e_steps: ∃e', e ⟶ e', from exists.intro (exp.ite e1' e2 e3) this,
+          show is_value e ∨ ∃e', e ⟶ e', from or.inr e_steps
+        )
       )
     )
-    (
-      assume e1 e2 e3: exp,
-      assume e1ih: is_val e1 ∨ step e1 ≠ none,
-      assume e2ih: is_val e2 ∨ step e2 ≠ none,
-      assume e3ih: is_val e3 ∨ step e3 ≠ none,
-      let e := ite e1 e2 e3 in
-      show is_val e ∨ step e ≠ none, from sorry
-    )
-    (
+    ( -- eq
       assume e1 e2: exp,
-      assume e1ih: is_val e1 ∨ step e1 ≠ none,
-      assume e2ih: is_val e2 ∨ step e2 ≠ none,
+      assume t: typ,
+      assume e1_typed_t: e1 ::: t,
+      assume e2_typed_t: e2 ::: t,
+      assume e1ih: is_value e1 ∨ ∃e1', e1 ⟶ e1',
+      assume e2ih: is_value e2 ∨ ∃e2', e2 ⟶ e2',
       let e := exp.eq e1 e2 in
-      show is_val e ∨ step e ≠ none, from sorry
+      have e_is_eq: e = exp.eq e1 e2, from rfl,
+      or.elim e1ih (
+        assume e1_is_val: is_value e1,
+        or.elim e2ih (
+          assume e2_is_val: is_value e2,
+          typ_cases t
+          ( -- num
+            assume t_is_num: t = typ.num,
+            have e1_typed_num: e1 ::: typ.num, by { rw[t_is_num] at e1_typed_t, assumption  },
+            have e2_typed_num: e2 ::: typ.num, by { rw[t_is_num] at e2_typed_t, assumption  },
+            have e1_exists_num: ∃n1: ℕ, e1 = exp.num n1, from numt_inversion e1_typed_num e1_is_val,
+            have e2_exists_num: ∃n2: ℕ, e2 = exp.num n2, from numt_inversion e2_typed_num e2_is_val,
+            exists.elim e1_exists_num (λn1, exists.elim e2_exists_num (λn2,
+              assume e2_is_num: e2 = exp.num n2,
+              assume e1_is_num: e1 = exp.num n1,
+              have exp.eq (exp.num n1) (exp.num n2) ⟶ exp.bool (n1 = n2), from step.eq_num,
+              have e ⟶ exp.bool (n1 = n2), by { rw [←e1_is_num, ←e2_is_num, ←e_is_eq] at this, assumption },
+              have e_steps: ∃e', e ⟶ e', from exists.intro (exp.bool (n1 = n2)) this,
+              show is_value e ∨ ∃e', e ⟶ e', from or.inr e_steps
+            ))
+          )
+          ( -- bool
+            assume t_is_bool: t = typ.bool,
+            have e1_typed_bool: e1 ::: typ.bool, by { rw[t_is_bool] at e1_typed_t, assumption  },
+            have e2_typed_bool: e2 ::: typ.bool, by { rw[t_is_bool] at e2_typed_t, assumption  },
+            have e1_some_bool: e1 = exp.bool true ∨ e1 = exp.bool false, from boolt_inversion e1_typed_bool e1_is_val,
+            have e2_some_bool: e2 = exp.bool true ∨ e2 = exp.bool false, from boolt_inversion e2_typed_bool e2_is_val,
+            or.elim e1_some_bool
+            (
+              assume e1_is_true: e1 = exp.bool true,
+              or.elim e2_some_bool
+              (
+                assume e2_is_true: e2 = exp.bool true,
+                have e_is_true_eq_true: e = exp.eq (exp.bool true) (exp.bool true),
+                by { rw [e1_is_true, e2_is_true] at e_is_eq, assumption },
+                have exp.eq (exp.bool true) (exp.bool true) ⟶ exp.bool true, from step.eq_bool,
+                have e ⟶ exp.bool true, by { rw [←e_is_true_eq_true] at this, assumption },
+                have e_steps: ∃e', e ⟶ e', from exists.intro (exp.bool true) this,
+                show is_value e ∨ ∃e', e ⟶ e', from or.inr e_steps
+              )
+              (
+                assume e2_is_false: e2 = exp.bool false,
+                have e_is_true_eq_false: e = exp.eq (exp.bool true) (exp.bool false),
+                by { rw [e1_is_true, e2_is_false] at e_is_eq, assumption },
+                have exp.eq (exp.bool true) (exp.bool false) ⟶ exp.bool false, from step.eq_bool,
+                have e ⟶ exp.bool false, by { rw [←e_is_true_eq_false] at this, assumption },
+                have e_steps: ∃e', e ⟶ e', from exists.intro (exp.bool false) this,
+                show is_value e ∨ ∃e', e ⟶ e', from or.inr e_steps
+              )
+            )
+            (
+              assume e1_is_false: e1 = exp.bool false,
+              or.elim e2_some_bool
+              (
+                assume e2_is_true: e2 = exp.bool true,
+                have e_is_false_eq_true: e = exp.eq (exp.bool false) (exp.bool true),
+                by { rw [e1_is_false, e2_is_true] at e_is_eq, assumption },
+                have exp.eq (exp.bool false) (exp.bool true) ⟶ exp.bool false, from step.eq_bool,
+                have e ⟶ exp.bool false, by { rw [←e_is_false_eq_true] at this, assumption },
+                have e_steps: ∃e', e ⟶ e', from exists.intro (exp.bool false) this,
+                show is_value e ∨ ∃e', e ⟶ e', from or.inr e_steps
+              )
+              (
+                assume e2_is_false: e2 = exp.bool false,
+                have e_is_false_eq_false: e = exp.eq (exp.bool false) (exp.bool false),
+                by { rw [e1_is_false, e2_is_false] at e_is_eq, assumption },
+                have exp.eq (exp.bool false) (exp.bool false) ⟶ exp.bool true, from step.eq_bool,
+                have e ⟶ exp.bool true, by { rw [←e_is_false_eq_false] at this, assumption },
+                have e_steps: ∃e', e ⟶ e', from exists.intro (exp.bool true) this,
+                show is_value e ∨ ∃e', e ⟶ e', from or.inr e_steps
+              )
+            )
+          )
+        )
+        (
+          assume e2_can_step: ∃e2', e2 ⟶ e2',
+          exists.elim e2_can_step (λe2', 
+            assume e2_steps: e2 ⟶ e2',
+            have e ⟶ exp.eq e1 e2', from step.eq_right e1_is_val e2_steps,
+            have e_steps: ∃e', e ⟶ e', from exists.intro (exp.eq e1 e2') this,
+            show is_value e ∨ ∃e', e ⟶ e', from or.inr e_steps
+          )
+        )
+      ) (
+        assume e1_can_step: ∃e1', e1 ⟶ e1',
+        exists.elim e1_can_step (λe1', 
+          assume e1_steps: e1 ⟶ e1',
+          have e ⟶ exp.eq e1' e2, from step.eq_left e1_steps,
+          have e_steps: ∃e', e ⟶ e', from exists.intro (exp.eq e1' e2) this,
+          show is_value e ∨ ∃e', e ⟶ e', from or.inr e_steps
+        )
+      )
     )
 
 end arith
